utp/examples/max_list.thy
@@ -1,5 +1,5 @@
 theory max_list
-  imports "UTP.utp_easy_parser"
+  imports "UTP.utp"
 begin
 
 alphabet max_st =
@@ -10,28 +10,28 @@ alphabet max_st =
 abbreviation maximum :: "nat list \<Rightarrow> max_st hrel"  where
   "maximum list \<equiv>
     xs := \<guillemotleft>list\<guillemotright> ;; 
-    if (#xs = 0)
+    if (length xs = 0)
     then 
       result := 0
     else
-      result := xs[0] ;;  
+      result := xs ! 0 ;;  
       i := 1 ;;
-      while i < #xs
-      invr xs = \<guillemotleft>list\<guillemotright> \<and> i > 0 \<and> result = Max(set(take(i, xs)))
+      while i < length xs
+      invr xs = \<guillemotleft>list\<guillemotright> \<and> i > 0 \<and> result = Max(set(take i xs))
       do
-        if xs[i] > result
-          then result := xs[i]  ;; i := i + 1
+        if xs ! i > result
+          then result := xs ! i  ;; i := i + 1
           else i := i + 1
         fi
       od
     fi"
 
 
-lemma "TRY(id \<Turnstile> maximum [4,3,7,1,12,8])"
+lemma "TRY(id\<^sub>s \<Turnstile> maximum [4,3,7,1,12,8])"
   apply (sym_eval)
   oops
 
-lemma "list \<noteq> [] \<Longrightarrow> {{true}} maximum list {{result = Max(set(\<guillemotleft>list\<guillemotright>))}}"
+lemma "list \<noteq> [] \<Longrightarrow> \<lbrace>true\<rbrace> maximum list \<lbrace>result = Max(set(\<guillemotleft>list\<guillemotright>))\<rbrace>\<^sub>u"
   apply (hoare_auto)
     apply (auto simp add: take_Suc_conv_app_nth)
   oops
